src/program_proof/ctrexample/server.v
@@ -337,6 +337,7 @@ Proof using Type*.
         apply nil_length_inv in HslSize.
         rewrite HslSize in Hbad.
         apply has_encoding_length in Hbad.
+        Transparent u64_le.
         simpl in Hbad.
         lia.
       }
